generic/Zeta.Generic.Thread.fsti
@@ -190,8 +190,15 @@ val evict_seq_invmap_monotonic (#vspec:_) (ep: epoch) (tl: verifiable_log vspec)
   : Lemma (ensures ((j1 < j2 ==> evict_seq_invmap ep tl j1 < evict_seq_invmap ep tl j2) /\
                     (j2 < j1 ==> evict_seq_invmap ep tl j2 < evict_seq_invmap ep tl j1)))
 
-val evict_elem_unique (#vspec:_) (tl: verifiable_log vspec) (i1 i2: (i: seq_index tl {is_blum_evict tl i}))
-  : Lemma (ensures (i1 <> i2 ==> blum_evict_elem tl i1 <> blum_evict_elem tl i2))
+val evict_elem_unique (#vspec:_) (ep: epoch) (tl: verifiable_log vspec) (i1 i2: SA.seq_index (evict_seq ep tl))
+  : Lemma (ensures (let es = evict_seq ep tl in
+                    i1 <> i2 ==>  S.index es i1 <> S.index es i2))
+
+val evict_elem_tid (#vspec:_) (ep: epoch) (tl: verifiable_log vspec) (i: SA.seq_index (evict_seq ep tl))
+  : Lemma (ensures (let es = evict_seq ep tl in
+                    let be = S.index es i in
+                    let t,_ = tl in
+                    be.tid = t))
 
 (* is the i'th entry an app function *)
 let is_appfn (#vspec:_) (tl: verifiable_log vspec) (i: seq_index tl)
